\section{Berechnung von $\kappa$}
\subsection{Schritt 1: Nenner $c^2a(1-e^2)$}
\[
c^2 = (2.99792458 \times 10^8)^2 = 8.987551787 \times 10^{16}\, \text{m}^2/\text{s}^2
\]
\[
a(1-e^2) = 5.545 \times 10^{10}\, \text{m}
\]
\[
c^2 a (1-e^2) = 4.9826 \times 10^{27}\, \text{m}^3/\text{s}^2
\]

\subsection{Schritt 2: ZÃ¤hler $6GM$}
\[
6GM = 7.964 \times 10^{20}\, \text{m}^3/\text{s}^2
\]

\subsection{Schritt 3: Berechnung von $\kappa$}
\[
\frac{6GM}{c^2 a (1-e^2)} = 1.5983 \times 10^{-7}
\]
\[
\kappa = \sqrt{1 - 1.5983 \times 10^{-7}} = 0.999999920085
\]