\section{Berechnung der Zeitableitungen}
\subsection{Radialgeschwindigkeit \( \dot{r} \)}
\[
\dot{r} = \frac{dr}{d\phi} \dot{\phi} = \left( \frac{a(1 - e^2) e \sin \phi}{(1 + e \cos \phi)^2} \right) \left( \frac{L}{m r^2} \right)
\]
Vereinfacht:
\[
\dot{r} = \frac{L e \sin \phi}{m a(1 - e^2)} (1 + e \cos \phi)
\]

\subsection{Radialbeschleunigung \( \ddot{r} \)}
\[
\ddot{r} = \frac{d}{d\phi} (\dot{r}) \cdot \dot{\phi}
\]
Mit ausf√ºhrlicher Ableitung:
\[
\ddot{r} = \frac{L^2 e (1 + e \cos \phi)^3}{m^2 a^3 (1 - e^2)^3} \left( \cos \phi + e \right)
\]