\section{Transformation: Heliozentrisch \textrightarrow\ Baryzentrisch}

\subsection*{Baryzentrische Position der Sonne}
\begin{equation}
\vec{R}_\odot = -\frac{\sum m_i \vec{r}_i}{M_\odot + \sum m_i}
\end{equation}

\subsection*{Baryzentrische Positionen der Planeten}
\begin{equation}
\vec{R}_i = \vec{R}_\odot + \vec{r}_i
\end{equation}

\subsection*{Baryzentrische Geschwindigkeiten}
\begin{align}
\vec{V}_\odot &= -\frac{\sum m_i \vec{v}_i}{M_\odot + \sum m_i} \\
\vec{V}_i &= \vec{V}_\odot + \vec{v}_i
\end{align}